---
title: "XOR of Consecutive Integers"
date: 2024-11-09
permalink: /posts/2024/11/bitwise/
tags:
  - bitwise operations
  - XOR
---

# Preliminaries

Let $A \oplus B$ be the bitwise XOR of $A$ and $B$.
For each pair of bits, the table below shows the result of XOR.

$$
\begin{array}{|c|c|c|}
\hline
A & B & A \oplus B \\
\hline
0 & 0 & 0 \\
0 & 1 & 1 \\
1 & 0 & 1 \\
1 & 1 & 0 \\
\hline
\end{array}
$$

This means that for any $A$, $A \oplus A = 0$ and $A \oplus 0 = A$.
In the context of bitwise operations, a number is the inverse of itself and 0 is the identity element.

# Properties

**Theorem 1** Let $A$ be an even natural.
Then, $A \oplus (A+1) = 1$.

**Proof**
Let $A$ be a natural
Then, $2\cdot A$ is $A$ with a 0 added to the right.
Similarly, $2\cdot A + 1$ is $A$ with a 1 added to the right.
Taking the XOR of $2\cdot A$ and $2\cdot A + 1$ gives us

$$
\begin{aligned}
2\cdot A \oplus (2\cdot A + 1) &= A0_2 \oplus A1_2 = 0\cdots 0 1 = 1.
\end{aligned}
$$

Thus, we have shown that the XOR of an even number and the next odd number is 1.

From here, we can extend this property to the XOR of 4 consecutive numbers.

**Theorem 2** Let $A$ be an even natural.
Then,

$$
\begin{aligned}
A \oplus (A+1) \oplus (A+2) \oplus (A+3) = 0
\end{aligned}
$$

**Proof**
By the previous theorem,

$$
\begin{aligned}
    (A+0) \oplus (A+1) &= 1 \\
    (A+2) \oplus (A+3) &= 1
\end{aligned}
$$

Then, $A \oplus (A+1) \oplus (A+2) \oplus (A+3) = 1 \oplus 1 = 0$.

**Theorem 3** Let $A$ be an odd natural.
Then, $A \oplus (A+1) = 2^n - 1$ where $n$ is some positive integer as described below.

**Proof** Since $A$ is odd, it must end in a 1 in binary.
Then, $A+1$ will be $A$ with the rightmost 0 flipped to a 1 and all the bits to the right of it flipped to 0.
Let $n$ be the position of such a bit.
The XOR of $A$ and $A+1$ of the bits before the $n$th bit will be 0 because they are the same.
The XOR of the $n$th bit will be 1 because they are different.
The XOR of the bits after the $n$th bit will be 1 because by definition of $n$, the bits in $A$ must all be 1 and the bits in $A+1$ must all be 0.
Thus, the XOR of $A$ and $A+1$ will be $2^n - 1$, or simply n 1s in binary.

**Theorem 4** Let $A$ be an odd natural.
Then,

$$
\begin{aligned}
    A \oplus (A+1) \oplus (A+2) \oplus (A+3) = 2^n - 4
\end{aligned}
$$

where $n$ is some positive integer as described below.

**Proof**
By the previous theorem,

$$
\begin{aligned}
(A+1) \oplus (A+2) \oplus (A+3) \oplus (A+4) &= 0
\end{aligned}
$$

Let $X$ be the XOR of the 4 consecutive numbers.
Then,

$$
\begin{aligned}
X &= A \oplus (A+1) \oplus (A+2) \oplus (A+3) \\
A \oplus (A+4) \oplus X &= A \oplus A \oplus (A+1) \oplus (A+2) \oplus (A+3) \oplus (A+4) \\
A \oplus (A+4) \oplus X &= 0 \\
X &= A \oplus (A+4)
\end{aligned}
$$

The proof is similar to the proof of Theorem 3, with only difference being that $n$ is the position of the rightmost $0$ in $A$ ignoring the last 2 bits.

**Definition**
Let $f(A): \mathbb{N}_0 \to \mathbb{N}_0$ be a function that returns the XOR of all numbers from $0$ to $A$ inclusive.
That is, $f(A) = 0 \oplus 1 \oplus 2 \oplus \cdots \oplus A$.

**Corollary** Let $A$ and $B$ be numbers such that $A < B$.
Then, $f(A-1) \oplus f(B) = A \oplus (A+1) \oplus \cdots \oplus B$.

# Generalization

**Theorem 5**
Let $A$ be a natural.
Then,

$$
\begin{aligned}
    f(A) &=
    \begin{cases}
        A & A \equiv 0 \pmod 4 \\
        1 & A \equiv 1 \pmod 4 \\
        A+1 & A \equiv 2 \pmod 4 \\
        0 & A \equiv 3 \pmod 4 \\
    \end{cases}
\end{aligned}
$$

**Proof**
The proof by cases is trivial with the theorems established above, and the theorem can also be used to prove all of the theorems above.
